# T\(n,k\)\= \(\(n\+k\)^2\-2\*\(n\+k\)\+4\-\(n\+3\*k\-2\)\*\(\-1\)^\(n\+k\)\)/2; n , k \> 0, read by antidiagonals\.
https://oeis.org/A221215
## JSON
```JSON
[1, 6, 5, 2, 3, 4, 15, 14, 13, 12, 7, 8, 9, 10, 11, 28, 27, 26, 25, 24, 23, 16, 17, 18, 19, 20, 21, 22, 45, 44, 43, 42, 41, 40, 39, 38, 29, 30, 31, 32, 33, 34, 35, 36, 37, 66, 65, 64, 63, 62, 61, 60, 59, 58, 57, 46, 47, 48, 49, 50, 51, 52, 53, 54, 55, 56, 91]
```
## Mathematica
```Mathematica
T[n_, k_] := ((n+k)^2 - 2(n+k) + 4 - (n+3k-2)(-1)^(n+k))/2;
```
```Mathematica
Table[T[n-k+1, k], {n, 1, 12}, {k, n, 1, -1}] // Flatten (* _Jean-Fran√ßois Alcover_, Jan 05 2019 *)
```
## Python
```Python
t=int((math.sqrt(8*n-7) - 1)/ 2)
i=n-t*(t+1)/2
j=(t*t+3*t+4)/2-n
result=((t+2)**2-2*(t+2)+4-(i+3*j-2)*(-1)**t)/2
```
