# Anti\-Fibonacci numbers: start with a\(0\) \= 0, and extend by the rule that the next term is the sum of the two smallest numbers that are not in the sequence nor were used to form an earlier sum\.
https://oeis.org/A075326
## JSON
```JSON
[0, 3, 9, 13, 18, 23, 29, 33, 39, 43, 49, 53, 58, 63, 69, 73, 78, 83, 89, 93, 98, 103, 109, 113, 119, 123, 129, 133, 138, 143, 149, 153, 159, 163, 169, 173, 178, 183, 189, 193, 199, 203, 209, 213, 218, 223, 229, 233, 238, 243, 249, 253, 258, 263, 269, 273, 279, 283]
```
## Maple
```Maple
# Maple code for M+1 terms of sequence, from _N. J. A. Sloane_, Oct 26 2014
c:=0; a:=[c]; t:=0; M:=100;
for n from 1 to M do
s:=t+1; if s in a then s:=s+1; fi;
t:=s+1; if t in a then t:=t+1; fi;
c:=s+t;
a:=[op(a),c];
od:
[seq(a[n],n=1..nops(a))];
```
## Mathematica
```Mathematica
(* Three sequences a,b,c as in Comments *)
z = 200;
mex[list_, start_] := (NestWhile[# + 1 &, start, MemberQ[list, #] &]);
a = {}; b = {}; c = {};
Do[AppendTo[a,
   mex[Flatten[{a, b, c}], If[Length[a] == 0, 1, Last[a]]]];
  AppendTo[b, mex[Flatten[{a, b, c}], Last[a]]];
  AppendTo[c, Last[a] + Last[b]], {z}];
Take[a, 100] (* A075425 *)
Take[b, 100] (* A047215 *)
Take[c, 100] (* A075326 *)
Grid[{Join[{"n"}, Range[0, 20]], Join[{"a(n)"}, Take[a, 21]],
  Join[{"b(n)"}, Take[b, 21]], Join[{"c(n)"}, Take[c, 21]]},
Alignment -> ".",
Dividers -> {{2 -> Red, -1 -> Blue}, {2 -> Red, -1 -> Blue}}]
(* _Peter J. C. Moses_, Apr 26 2018 *)
********
(* Sequence "a" via A035263 substitutions *)
Accumulate[Prepend[Flatten[Nest[Flatten[# /. {0 -> {1, 1}, 1 -> {1, 0}}] &, {0}, 7] /. Thread[{0, 1} -> {{5, 5}, {6, 4}}]], 3]]
(* _Peter J. C. Moses_, May 01 2018 *)
********
(* Sequence "a" via Hofstadter substitutions; see his 2014 link *)
morph = Rest[Nest[Flatten[#/.{1->{3},3->{1,1,3}}]&,{1},6]]
hoff = Accumulate[Prepend[Flatten[morph/.Thread[{1,3}->{{6,4,5,5},{6,4,6,4,6,4,5,5}}]],3]]
(* _Peter J. C. Moses_, May 01 2018 *)
```
## Haskell
```Haskell
import Data.List ((\\))
a075326 n = a075326_list !! n
a075326_list = 0 : f [1..] where
   f ws@(u:v:_) = y : f (ws \\ [u, v, y]) where y = u + v
-- _Reinhard Zumkeller_, Oct 26 2014
```
## Python
```Python
def aupton(nn):
    alst, disallowed, mink = [0], {0}, 1
    for n in range(1, nn+1):
        nextk = mink + 1
        while nextk in disallowed: nextk += 1
        an = mink + nextk
        alst.append(an)
        disallowed.update([mink, nextk, an])
        mink = nextk + 1
        while mink in disallowed: mink += 1
    return alst
print(aupton(57)) # _Michael S. Branicky_, Jan 31 2022
```
```Python
def A075326(n): return 5*n-1-int((n|(~((m:=n-1>>1)+1)&m).bit_length())&1) if n else 0 # _Chai Wah Wu_, Sep 11 2024
```
