# T\(n,k\) \= \(k \+ 3\*n \- 2 \- \(k\+n\-2\)\*\(\-1\)^\(k\+n\)\)/2 n, k \> 0, read by antidiagonals\.
https://oeis.org/A210530
## JSON
```JSON
[1, 2, 3, 1, 2, 3, 4, 5, 6, 7, 1, 2, 3, 4, 5, 6, 7, 8, 9, 10, 11, 1, 2, 3, 4, 5, 6, 7, 8, 9, 10, 11, 12, 13, 14, 15, 1, 2, 3, 4, 5, 6, 7, 8, 9, 10, 11, 12, 13, 14, 15, 16, 17, 18, 19, 1, 2, 3, 4, 5, 6, 7, 8, 9, 10, 11, 12, 13, 14, 15, 16, 17, 18, 19, 20, 21, 22]
```
## Mathematica
```Mathematica
T[n_, k_] := (k+3n-2-(k+n-2)(-1)^(k+n))/2; Table[T[n-k+1, k], {n, 1, 12}, {k, n, 1, -1}] // Flatten (* _Jean-Fran√ßois Alcover_, Nov 17 2018 *)
```
## PARI
```PARI
T(n,k) = (k+3*n-2-(k+n-2)*(-1)^(k+n))/2; \\ _Andrew Howroyd_, Jan 11 2018
```
## Python
```Python
t=int((math.sqrt(8*n-7)-1)/2)
v=int((t+2)/2)
result=n-v*(2*v-3)-1
```
