# T\(n,k\) \= \(\(k\+n\)^2 \- 4\*k \+ 3 \- \(\-1\)^n \- \(k\+n\)\*\(\-1\)^\(k\+n\)\)/2; n, k \> 0, read by antidiagonals\.
https://oeis.org/A213171
## JSON
```JSON
[1, 4, 5, 2, 3, 6, 9, 10, 13, 14, 7, 8, 11, 12, 15, 18, 19, 22, 23, 26, 27, 16, 17, 20, 21, 24, 25, 28, 31, 32, 35, 36, 39, 40, 43, 44, 29, 30, 33, 34, 37, 38, 41, 42, 45, 48, 49, 52, 53, 56, 57, 60, 61, 64, 65, 46, 47, 50, 51, 54, 55, 58, 59, 62, 63, 66, 69]
```
## Maple
```Maple
T:=(n,k)->((k+n)^2-4*k+3-(-1)^n-(k+n)*(-1)^(k+n))/2: seq(seq(T(k,n-k),k=1..n-1),n=1..13); # _Muniru A Asiru_, Dec 06 2018
```
## Mathematica
```Mathematica
T[n_, k_] := ((n+k)^2 - 4k + 3 - (-1)^n - (-1)^(n+k)(n+k))/2;
```
```Mathematica
Table[T[n-k+1, k], {n, 1, 12}, {k, n, 1, -1}] // Flatten (* _Jean-Fran√ßois Alcover_, Dec 06 2018 *)
```
## Python
```Python
t=int((math.sqrt(8*n-7) - 1)/ 2)
i=n-t*(t+1)/2
j=(t*t+3*t+4)/2-n
result=((t+2)**2-4*j+3-(-1)**i-(t+2)*(-1)**t)/2
```
