# a\(1\) \= 1; for n \> 1, a\(n\) \= a\(n\-1\)\-\(n\+1\) if this is positive and has not already appeared in the sequence, otherwise a\(n\) \= a\(n\-1\)\+\(n\+1\)\.
https://oeis.org/A066199
## JSON
```JSON
[1, 4, 8, 3, 9, 2, 10, 19, 29, 18, 6, 19, 5, 20, 36, 53, 35, 16, 36, 15, 37, 14, 38, 13, 39, 12, 40, 11, 41, 72, 104, 71, 105, 70, 34, 71, 33, 72, 32, 73, 31, 74, 30, 75, 121, 168, 120, 169, 119, 68, 120, 67, 121, 66, 122, 65, 7, 66, 126, 187, 125, 62, 126, 61, 127, 60, 128]
```
## Python
```Python
l=[0, 1]
for n in range(2, 101):
    x=l[n - 1] - (n + 1)
    if x>0 and x not in l: l.append(x)
    else: l.append(l[n - 1] + (n + 1))
print(l[1:]) # _Indranil Ghosh_, Jun 02 2017
```
