# a\(2n\) \= a\(n\-1\) \+ a\(n\) and a\(2n\+1\) \= a\(n\+1\) for n\>\=1, with a\(0\)\=1, a\(1\)\=2\.
https://oeis.org/A214127
## JSON
```JSON
[1, 2, 3, 3, 5, 3, 6, 5, 8, 3, 8, 6, 9, 5, 11, 8, 13, 3, 11, 8, 11, 6, 14, 9, 15, 5, 14, 11, 16, 8, 19, 13, 21, 3, 16, 11, 14, 8, 19, 11, 19, 6, 17, 14, 20, 9, 23, 15, 24, 5, 20, 14, 19, 11, 25, 16, 27, 8, 24, 19, 27, 13, 32, 21, 34, 3, 24, 16, 19, 11, 27, 14, 25]
```
## Mathematica
```Mathematica
t = {1, 2}; Do[If[EvenQ[n], AppendTo[t, t[[n/2]] + t[[n/2 + 1]]], AppendTo[t, t[[(n + 3)/2]]]], {n, 2, 100}]; t (* _T. D. Noe_, Jul 11 2012 *)
```
## Python
```Python
a = [1]*(77*2)
a[1]=2
for n in range(1,77):
    a[2*n  ]=a[n-1]+a[n]
    a[2*n+1]=a[n+1]
    print(str(a[n-1]),end=',')
```
