# a\(\-1\) \= 1 and g\.f\. A\(x\) satisfies A\(x\) \- 1/A\(x\) \= 1/x \- 1\.
https://oeis.org/A214649
## JSON
```JSON
[1, -1, 1, 1, 0, -2, -3, 1, 11, 15, -13, -77, -86, 144, 595, 495, -1520, -4810, -2485, 15675, 39560, 6290, -159105, -324805, 87075, 1592843, 2616757, -2136539, -15726114, -20247800, 32296693, 152909577, 145139491, -417959049, -1460704685, -885536173]
```
## Maple
```Maple
A214649 := n -> `if`(n<2, (-1)^(n-1), simplify(hypergeom([(1-n)/2, 1-n/2], [2], -4))): seq(A214649(n), n=-1..34); # _Peter Luschny_, May 28 2014
```
## Mathematica
```Mathematica
CoefficientList[Series[(1-x + Sqrt[1-2*x+5*x^2])/2, {x, 0, 50}], x] (* _G. C. Greubel_, Aug 10 2018 *)
```
## PARI
```PARI
{a(n) = if( n<-1, 0, polcoeff( ( 1 - x + sqrt( 1 - 2*x + 5*x^2 + x^2 * O(x^n) ) ) / ( 2*x ), n))}
```
```PARI
{a(n) = local( A ); if( n<-1, 0, A = 1 / x + O(x^0); forstep( k = -1, n, 2, A = 1 / x - 1 + 1 / A ); polcoeff( A, n ) )};
```
## Maxima
```Maxima
a(n):=if n=-1 then 1 else sum(((-1)^(j-1)*binomial(2*j-1,j)*binomial(n-1,2*j-2))/(2*j-1),j,0,(n+1)/2); /* _Vladimir Kruchinin_, May 28 2014 */
```
## Magma
```Magma
m:=50; R<x>:=PowerSeriesRing(Rationals(), m); Coefficients(R!((1-x + Sqrt(1-2*x+5*x^2))/2)); // _G. C. Greubel_, Aug 10 2018
```
## Python
```Python
A214649 = [1, -1, 1]
for n in range(2, 802):
    A214649.append( ((2*n-1)*A214649[-1]
      - 5*(n-2)*A214649[-2])//(n+1) )
for n in range(802):
    print(n-1, A214649[n]) # _Gennady Eremin_, May 18 2021
```
