# a\(2n\)\=a\(n\-1\)\+a\(n\) and a\(2n\+1\)\=a\(n\+1\) for n\>\=1, with a\(0\)\=a\(1\)\=1\.
https://oeis.org/A214126
## JSON
```JSON
[1, 1, 2, 2, 3, 2, 4, 3, 5, 2, 5, 4, 6, 3, 7, 5, 8, 2, 7, 5, 7, 4, 9, 6, 10, 3, 9, 7, 10, 5, 12, 8, 13, 2, 10, 7, 9, 5, 12, 7, 12, 4, 11, 9, 13, 6, 15, 10, 16, 3, 13, 9, 12, 7, 16, 10, 17, 5, 15, 12, 17, 8, 20, 13, 21, 2, 15, 10, 12, 7, 17, 9, 16, 5, 14, 12]
```
## Maple
```Maple
a:= proc(n) local r;
      a(n):= `if`(n<2, 1, `if`(irem(n, 2, 'r')=0, a(r-1)+a(r), a(r+1)))
    end:
seq(a(n), n=1..100);  # _Alois P. Heinz_, Jul 06 2012
```
## Mathematica
```Mathematica
a[0] = a[1] = 1;
```
```Mathematica
a[n_] := a[n] = If[EvenQ[n], a[n/2-1] + a[n/2], a[(n-1)/2+1]];
```
```Mathematica
Array[a, 100, 0] (* _Jean-FranÃ§ois Alcover_, May 31 2019 *)
```
## Python
```Python
a = [1]*(77*2)
for n in range(1,77):
    a[2*n  ]=a[n-1]+a[n]
    a[2*n+1]=a[n+1]
    print(str(a[n-1]),end=',')
```
