# a\(n\) \= Sum\_\{k\=0\.\.n\} \(\-k\)^k\.
https://oeis.org/A326501
## JSON
```JSON
[1, 0, 4, -23, 233, -2892, 43764, -779779, 15997437, -371423052, 9628576948, -275683093663, 8640417354593, -294234689237660, 10817772136320356, -427076118244539019, 18019667955465012597, -809220593930871751580, 38537187481365665823844]
```
## Maple
```Maple
a:= proc(n) option remember; `if`(n<0, 0, (-n)^n+a(n-1)) end:
seq(a(n), n=0..23);  # _Alois P. Heinz_, Sep 12 2019
```
## Mathematica
```Mathematica
RecurrenceTable[{a[0] == 1, a[n] == a[n-1] + (-n)^n}, a, {n, 0, 23}] (* _Jean-FranÃ§ois Alcover_, Nov 27 2020 *)
```
## PARI
```PARI
{a(n) = sum(k=0, n, (-k)^k)}
```
## Python
```Python
from itertools import accumulate, count, islice
def A326501_gen(): # generator of terms
    yield from accumulate((-k)**k for k in count(0))
A326501_list = list(islice(A326501_gen(),10)) # _Chai Wah Wu_, Jun 18 2022
```
