# a\(n\) \= Sum\_\{k \= 0\.\.n\} \(\-1\)^k\*k^3\*binomial\(n,k\)^3\.
https://oeis.org/A273630
## JSON
```JSON
[0, -1, 0, 162, 0, -11250, 0, 576240, 0, -25259850, 0, 1007242236, 0, -37685439792, 0, 1346871240000, 0, -46504059326010, 0, 1562983866658500, 0, -51407781284599740, 0, 1661123953798807680, 0, -52886433789393750000, 0, 1662782404368229351200]
```
## Maple
```Maple
seq(add((-1)^k*k^3*binomial(n,k)^3, k = 0..n), n = 0..30);
```
## Mathematica
```Mathematica
Table[Sum[(-1)^k*k^3 Binomial[n, k]^3, {k, 0, n}], {n, 0, 27}] (* _Michael De Vlieger_, Jul 22 2016 *)
```
## PARI
```PARI
a(n) = sum(k=0, n, (-1)^k*k^3*binomial(n, k)^3) \\ _Felix FrÃ¶hlich_, Jul 22 2016
```
## Magma
```Magma
[&+[(-1)^k*k^3 *Binomial(n, k)^3: k in [0..n]]: n in [0..70]]; // _Vincenzo Librandi_, Jul 23 2016
```
## Python
```Python
from math import factorial
def A273630(n): return (1 if (m:=n>>1)&1 else -1)*n**3*factorial(3*m)//factorial(m)**3 if n&1 else 0 # _Chai Wah Wu_, Oct 04 2022
```
