# a\(n\) \= Sum\_\{k \= 0\.\.n\} \(\-1\)^k\*binomial\(k,2\)^3\*binomial\(n,k\)^3\.
https://oeis.org/A273631
## JSON
```JSON
[0, 0, 1, 0, -1296, 0, 303750, 0, -36879360, 0, 3157481250, 0, -217564322976, 0, 12926105848656, 0, -689598074880000, 0, 33901459248661290, 0, -1562983866658500000, 0, 68423756889802253940, 0, -2870422192164339671040, 0, 116191495035298068750000]
```
## Maple
```Maple
seq(add((-1)^k*binomial(k,2)^3*binomial(n,k)^3, k = 0..n), n = 0..30);
```
## Mathematica
```Mathematica
Table[Sum[(-1)^k*Binomial[k, 2]^3 Binomial[n, k]^3, {k, 0, n}], {n, 0, 27}] (* _Michael De Vlieger_, Jul 22 2016 *)
```
## PARI
```PARI
a(n) = sum(k=0, n, (-1)^k*binomial(k, 2)^3*binomial(n, k)^3) \\ _Felix FrÃ¶hlich_, Jul 22 2016
```
## Magma
```Magma
[&+[(-1)^k*Binomial(k,2)^3*Binomial(n,k)^3: k in [0..n]]: n in [0..70]]; // _Vincenzo Librandi_, Jul 23 2016
```
## Python
```Python
from math import factorial
def A273631(n): return 0 if n&1 or n == 0 else (-1 if (m:=n-1>>1)&1 else 1)*((m+1)*(n-1))**3*factorial(3*m)//factorial(m)**3 # _Chai Wah Wu_, Oct 04 2022
```
