# a\(0\) \= 0; thereafter, a\(2\*n\+1\) \= a\(n\)\+2\*n\+1, otherwise a\(n\) \= n\.
https://oeis.org/A274593
## JSON
```JSON
[0, 1, 2, 4, 4, 7, 6, 11, 8, 13, 10, 18, 12, 19, 14, 26, 16, 25, 18, 32, 20, 31, 22, 41, 24, 37, 26, 46, 28, 43, 30, 57, 32, 49, 34, 60, 36, 55, 38, 71, 40, 61, 42, 74, 44, 67, 46, 88, 48, 73, 50, 88, 52, 79, 54, 101, 56, 85, 58, 102]
```
## Maple
```Maple
f:= proc(n) option remember; if n::even then n else n + procname((n-1)/2) fi end proc:
map(f, [$0..100]); # _Robert Israel_, Jul 04 2016
```
## Mathematica
```Mathematica
a[0] = 0; a[n_] := a[n] = If[OddQ@ n, a[#] + 2 # + 1 &[(n - 1)/2], n]; Table[a@ n, {n, 0, 59}] (* _Michael De Vlieger_, Jul 04 2016 *)
```
## Python
```Python
def A274593(n): return (((m:=~(n+1)&n)<<1)+1)*((n>>(k:=m.bit_length()))|1)-k-1 # _Chai Wah Wu_, Jul 13 2022
```
