# a\(n\) \= a\(n\-1\) \- n\*a\(n\-2\); a\(0\) \= a\(1\) \= 1\.
https://oeis.org/A286032
## JSON
```JSON
[1, 1, -1, -4, 0, 20, 20, -120, -280, 800, 3600, -5200, -48400, 19200, 696800, 408800, -10740000, -17689600, 175630400, 511732800, -3000875200, -13747264000, 52271990400, 368459062400, -886068707200, -10097545267200, 12940241120000, 285573963334400]
```
## Maple
```Maple
a := proc(n) option remember;
if n <= 1 then 1 else a(n-1) - n*a(n-2) fi end:
seq(a(n), n = 0..27);
a_list := proc(len) 1 - sqrt(Pi/2)*exp(-((x-1)^2)/2)*(x-1)*
(erfi((x-1)/sqrt(2)) + erfi(1/sqrt(2))); series(%, x, len+2):
seq(n!*simplify(coeff(%,x,n)),n=0..len-1) end: a_list(27);
```
## Mathematica
```Mathematica
l={1, 1}; Do[AppendTo[l, l[[-1]] - n*l[[-2]]], {n, 2, 30}]; l (* _Indranil Ghosh_, May 01 2017 *)
```
```Mathematica
RecurrenceTable[{a[0]==a[1]==1,a[n]==a[n-1]-n a[n-2]},a,{n,40}] (* _Harvey P. Dale_, Jun 20 2021 *)
```
## Python
```Python
l=[1, 1]
a=b=1
i=2
while i<=30:
    l.append(b - i*a)
    b=l[-1]
    a=l[-2]
    i+=1
print(l) # _Indranil Ghosh_, May 01 2017
```
