# a\(1\) \= 0, and for n \> 1, a\(n\) \= A286105\(A285735\(n\)\) \- A286105\(A285734\(n\)\)\.
https://oeis.org/A286106
## JSON
```JSON
[0, 0, 1, 0, 1, 0, 2, 1, 1, 0, 0, 0, 1, 0, 1, 1, 0, 0, 2, 0, 0, 0, 1, 1, 1, 0, 0, 0, 0, 0, 0, 0, 1, 0, 0, 1, 0, 0, 0, -1, -1, 0, 0, 0, 1, 0, 1, 1, 0, 1, 1, 0, 0, 0, 0, 0, 0, 0, 0, 0, 0, 0, 1, 1, 0, 0, -1, 0, 0, 0, 0, 0, 1, 0, 1, 0, -1, 0, 0, 1, 0, 0, -1, 0, 0, 0, 0, 1, 1, 1, 0, 0, 0, 0, 1, 1, 0, 0, 0, 0, 0, 0, 0, 0, 0, 0, 0, 0, 0, 0, 0, 0, 0, 0, 0, 0, 0, 0, 0]
```
## Scheme
```Scheme
(define (A286106 n) (if (= 1 n) 0 (- (A286105 (A285735 n)) (A286105 (A285734 n)))))
```
## Python
```Python
from sympy.ntheory.factor_ import core
def issquarefree(n): return core(n) == n
def a285734(n):
    if n==1: return 0
    j=n//2
    while True:
        if issquarefree(j) and issquarefree(n - j): return j
        else: j-=1
def a285735(n): return n - a285734(n)
def a286105(n): return 0 if n==1 else 1 + max(a286105(a285734(n)), a286105(a285735(n)))
def a286106(n): return 0 if n==1 else a286105(a285735(n)) - a286105(a285734(n))
print([a286106(n) for n in range(1, 121)]) # _Indranil Ghosh_, May 02 2017
```
