# a\(n\) \= n^n \- a\(n\-1\), with a\(1\) \= 1\.
https://oeis.org/A001099
## JSON
```JSON
[1, 3, 24, 232, 2893, 43763, 779780, 15997436, 371423053, 9628576947, 275683093664, 8640417354592, 294234689237661, 10817772136320355, 427076118244539020, 18019667955465012596, 809220593930871751581, 38537187481365665823843, 1939882468178947923300136]
```
## Mathematica
```Mathematica
Abs[Table[Sum[k^k*(-1)^(k+1),{k,1,n}],{n,1,30}]] (* _Alexander Adamchuk_, Jun 30 2006 *)
```
```Mathematica
RecurrenceTable[{a[1]==1,a[n]==n^n-a[n-1]},a,{n,20}] (* _Harvey P. Dale_, Jan 21 2015 *)
```
## Python
```Python
from itertools import accumulate, count, islice
def A001099_gen(): # generator of terms
    yield from accumulate((k**k for k in count(1)),func=lambda x,y:y-x)
A001099_list = list(islice(A001099_gen(),20)) # _Chai Wah Wu_, Jun 17 2022
```
