# For a string of letters of length k, say abc\.\.\.def, let f\(k\) be the string of length k\-1 consisting of the adjacent pairs ab, bc, cd, \.\.\., de, ef\. Given n, let U be the string of length 2n consisting of n 1's followed by n 2's: 11\.\.\.122\.\.\.2\. Then a\(n\) is the number of the C\(2n,n\) permutations V of U such that f\(U\) and f\(V\) agree in exactly one place\.
https://oeis.org/A098813
## JSON
```JSON
[1, 1, 4, 19, 57, 178, 543, 1591, 4598, 13117, 36999, 103514, 287653, 794847, 2186054, 5988339, 16347999, 44497490, 120804023, 327217525, 884531586, 2386747391, 6429784509, 17296261734, 46465809007, 124678595953, 334173980818, 894778164125]
```
## Maple
```Maple
with(combinat): for n from 1 to 10 do y:=0:B:=array: M:=[seq(11,i=1..n-1),seq(12,i=n),seq(22,i=n+1..2*n-1)]: S:=[seq(i,i=1..2*n)]: L:=choose(S,n): for j from 1 to binomial(2*n,n) do for k from 1 to 2*n-1 do if member(k,L[j]) then B[k]:=10 else B[k]:=20 end if: if member(k+1,L[j]) then B[k]:=B[k]+1 else B[k]:=B[k]+2 end if end do: x:=0: for l from 1 to 2*n-1 do if B[l]=M[l] then x:=x+1 end if end do: if x=1 then y:=y+1 end if end do: print(y) end do: # _Miklos Kristof_, Oct 07 2004
```
## Python
```Python
def find(bits_in, n0, n1, match):
....global count, U
....bitsleft = n0 + n1
....if bitsleft==0:
........if match:
............count += 1
....else:
........bitsleft -= 1
........if n0 > 0:
............bits_out = bits_in<<1
............new_match = (bits_out&3) == ((U >> bitsleft)&3)
............if not (match and new_match):
................find(bits_out, n0-1, n1, match or new_match)
........if n1 > 0:
............bits_out = (bits_in<<1)|1;
............new_match = (bits_out&3) == ((U >> bitsleft)&3)
............if not (match and new_match):
................find(bits_out, n0, n1-1, match or new_match)
def A098813(n):
....global count, U
....count = 0 ; U = (1<<n)-1
....find(0, n-1, n, False)
....find(1, n, n-1, False)
....return count
# _Bert Dobbelaere_, Dec 23 2018
```
