# a\(0\) \= 0; thereafter a\(n\) \= a\(n\-1\)/2 \+ n if a\(n\-1\) is even, otherwise a\(n\) \= a\(n\-1\) \+ a\(n\-2\)\.
https://oeis.org/A350129
## JSON
```JSON
[0, 1, 1, 2, 5, 7, 12, 13, 25, 38, 29, 67, 96, 61, 157, 218, 125, 343, 468, 253, 721, 974, 509, 1483, 1992, 1021, 3013, 4034, 2045, 6079, 8124, 4093, 12217, 16310, 8189, 24499, 32688, 16381, 49069, 65450, 32765, 98215, 130980, 65533, 196513, 262046, 131069, 393115, 524184]
```
## Mathematica
```Mathematica
a[0] = 0; a[n_] := a[n] = If[EvenQ[a[n - 1]], a[n - 1]/2 + n, a[n - 1] + a[n - 2]]; Array[a, 50, 0] (* _Amiram Eldar_, Dec 15 2021 *)
```
## Python
```Python
a = [0]
[a.append(a[-1] + a[-2] if a[-1]%2 else a[-1]//2 + n) for n in range(1, 49)]
print(a) # _Michael S. Branicky_, Dec 15 2021
```
## PARI
```PARI
seq(n)={my(a=vector(n)); a[1]=0; for(n=2, #a, a[n] = if(a[n-1]%2==0, a[n-1]/2+(n-1), a[n-1]+a[n-2])); a} \\ _Andrew Howroyd_, Dec 15 2021
```
```PARI
concat([0], Vec((1 + 2*x^3)*(1 + x + 2*x^2 - x^3 + x^4)/((1 - x)^2*(1 + x + x^2)^2*(1 - 2*x^3)) + O(x^30))) \\ _Andrew Howroyd_, Dec 15 2021
```
