# a\(n\) \= Sum\_\{k\=1\.\.n\} Sum\_\{d\=1\.\.k\} \(k mod d\)\.
https://oeis.org/A072481
## JSON
```JSON
[0, 0, 0, 1, 2, 6, 9, 17, 25, 37, 50, 72, 89, 117, 148, 184, 220, 271, 318, 382, 443, 513, 590, 688, 773, 876, 988, 1113, 1237, 1388, 1526, 1693, 1860, 2044, 2241, 2459, 2657, 2890, 3138, 3407, 3665, 3962, 4246, 4571, 4899, 5238, 5596, 5999, 6373, 6787, 7207]
```
## Maple
```Maple
N:= 200: # to get a(0) to a(N)
S:= series(add(k*x^(2*k)/(1-x^k),k=1..floor(N/2))/(1-x)^2, x, N+1):
seq((n^3-n)/6 - coeff(S,x,n), n=0..N); # _Robert Israel_, Aug 13 2015
```
## Mathematica
```Mathematica
a[n_] := n(n+1)(2n+1)/6 - Sum[DivisorSigma[1, k] (n-k+1), {k, 1, n}];
```
```Mathematica
Table[a[n], {n, 0, 50}] (* _Jean-Fran√ßois Alcover_, Mar 08 2019, after _Omar E. Pol_ *)
```
## Python
```Python
for n in range(99):
    s = 0
    for k in range(1,n+1):
      for d in range(1,k+1):
        s += k % d
    print(str(s), end=',')
```
```Python
from math import isqrt
def A072481(n): return (n*(n+1)*((n<<1)+1)-((s:=isqrt(n))**2*(s+1)*((s+1)*((s<<1)+1)-6*(n+1))>>1)-sum((q:=n//k)*(-k*(q+1)*(3*k+(q<<1)+1)+3*(n+1)*((k<<1)+q+1)) for k in range(1,s+1)))//6 # _Chai Wah Wu_, Oct 22 2023
```
## PARI
```PARI
a(n) = sum(k=1, n, sum(d=1, k, k % d)); \\ _Michel Marcus_, Feb 11 2014
```
