# a\(1\) \= 0; a\(2\) \= 1; thereafter a\(n\) \= a\(n\-1\)/2 if a\(n\-1\) is even, otherwise a\(n\) \= a\(n\-1\) \+ a\(\(n\-1\)\-a\(n\-1\)\)\.
https://oeis.org/A352840
## JSON
```JSON
[0, 1, 1, 2, 1, 3, 4, 2, 1, 3, 7, 9, 10, 5, 6, 3, 13, 15, 16, 8, 4, 2, 1, 3, 7, 22, 11, 14, 7, 9, 13, 28, 14, 7, 18, 9, 20, 10, 5, 12, 6, 3, 8, 4, 2, 1, 3, 7, 13, 22, 11, 23, 30, 15, 20, 10, 5, 28, 14, 7, 37, 40, 20, 10, 5, 12, 6, 3, 8, 4, 2, 1, 3, 7, 13, 53]
```
## Python
```Python
result = [0, 1]
iterations = 100
for i in range(1, iterations):
    if result[i]%2 == 0:
        result.append(result[i] // 2)
    else:
        result.append(result[i] + result[i - result[i]])
print(result, end='', sep=' ')
```
## MATLAB
```MATLAB
result = [0 1];
iterations = 100;
for i = 2:iterations
    if mod(result(i), 2) == 0
        result(i+1) = int32(result(i)/2);
    else
        result(i+1) = (result(i) + result(i - result(i)));
    end
end
```
