# a\(n\) \= Sum\_\{k \= 0\.\.n\-1\} binomial\(n,k\)\*binomial\(n\-1,k\)\*binomial\(n\+k,k\)\*binomial\(n\-1\+k,k\)\.
https://oeis.org/A352653
## JSON
```JSON
[0, 1, 13, 253, 5741, 142001, 3713305, 100961365, 2825369965, 80843126905, 2354354542013, 69555586698533, 2079506849058809, 62797822901091409, 1912714261589863633, 58691012753161717253, 1812592783819686728045, 56298976785759622597385, 1757493098495181029912485]
```
## Maple
```Maple
seq(add(binomial(n,k)^2*binomial(n+k-1,k-1)^2, k = 1..n), n = 0..20);
```
## Mathematica
```Mathematica
a[n_] := n^2 HypergeometricPFQ[{1 - n, 1 - n, 1 + n, 1 + n}, {1, 2, 2}, 1];
```
```Mathematica
Table[a[n], {n, 0, 18}] (* _Peter Luschny_, Apr 17 2022 *)
```
## PARI
```PARI
a(n) = sum(k=1, n, binomial(n,k)^2*binomial(n+k-1,k-1)^2); \\ _Michel Marcus_, Apr 19 2022
```
## Python
```Python
def A352653(n):
    if n == 0: return 0
    m, g = 1, 0
    for k in range(n+1):
        g += m*n**2//(n+k)**2
        m *= ((n+k+1)*(n-k))**2
        m //= (k+1)**4
    return g>>1 # _Chai Wah Wu_, Oct 03 2022
```
