# a\(n\+1\) \= Sum\_\{k\=1\.\.n\} \(a\(k\) \+ k\*\(n\-k\)\), with a\(1\)\=1\.
https://oeis.org/A335927
## JSON
```JSON
[1, 2, 7, 20, 50, 115, 251, 530, 1096, 2237, 4529, 9124, 18326, 36743, 73591, 147302, 294740, 589633, 1179437, 2359064, 4718338, 9436907, 18874067, 37748410, 75497120, 150994565, 301989481, 603979340, 1207959086]
```
## Mathematica
```Mathematica
a[1] = 1; a[n_] := a[n] = Sum[a[k] + k*(n - k), {k, 1, n - 1}]; Array[a, 30] (* _Amiram Eldar_, Jul 02 2020 *)
```
```Mathematica
LinearRecurrence[{5,-9,7,-2},{1,2,7,20,50},30] (* _Harvey P. Dale_, Sep 27 2024 *)
```
## Python
```Python
def a(n):
    if n == 1: return 1
    return sum([a(k) + k*(n-k) for k in range(1,n)])
```
