# a\(n\) \= 3\*a\(n\-2\) \- a\(n\-1\) for n \> 1, a\(0\) \= 0, a\(1\) \= 1\.
https://oeis.org/A182228
## JSON
```JSON
[0, 1, -1, 4, -7, 19, -40, 97, -217, 508, -1159, 2683, -6160, 14209, -32689, 75316, -173383, 399331, -919480, 2117473, -4875913, 11228332, -25856071, 59541067, -137109280, 315732481, -727060321, 1674257764, -3855438727, 8878212019, -20444528200, 47079164257, -108412748857]
```
## Mathematica
```Mathematica
RecurrenceTable[{a[n]== - a[n-1] + 3*a[n-2], a[0]== 0, a[1]== 1}, a, {n,0,200}] (* _G. C. Greubel_, Aug 30 2015 *)
```
```Mathematica
LinearRecurrence[{-1,3},{0,1},40] (* _Harvey P. Dale_, Oct 23 2016 *)
```
## Python
```Python
prpr = 0
prev = 1
for i in range(2,55):
    current = prpr*3-prev
    print (current, end=',')
    prpr = prev
    prev = current
```
## Magma
```Magma
[n le 2 select n-1 else -Self(n-1) + 3*Self(n-2): n in [1..40]]; // _Vincenzo Librandi_, Aug 31 2015
```
