# a\(0\)\=0, a\(1\)\=1, a\(n\) \= \(a\(n\-2\)\*a\(n\-1\)\+1\) mod n\.
https://oeis.org/A182457
## JSON
```JSON
[0, 1, 1, 2, 3, 2, 1, 3, 4, 4, 7, 7, 2, 2, 5, 11, 8, 4, 15, 4, 1, 5, 6, 8, 1, 9, 10, 10, 17, 26, 23, 10, 7, 5, 2, 11, 23, 32, 15, 13, 36, 18, 19, 42, 7, 25, 38, 11, 35, 43, 6, 4, 25, 48, 13, 20, 37, 0, 1, 1, 2, 3, 7, 22, 27, 10, 7, 4, 29, 48, 63, 43, 46, 8]
```
## Mathematica
```Mathematica
Nest[Append[#, Mod[#[[-1]]*#[[-2]] + 1, Length[#] + 1]] &, {1, 1}, 71] (* _Ivan Neretin_, May 14 2015 *)
```
## Python
```Python
prpr = 0
prev = 1
for n in range(2,77):
.  current = ( prev*prpr + 1 ) % n
.  print prpr,
.  prpr = prev
.  prev = current
```
