# a\(n\+1\) \= a\(\|n\-a\(n\)^2\|\) \+ 1, a\(0\) \= 0\.
https://oeis.org/A364197
## JSON
```JSON
[0, 1, 1, 2, 2, 1, 3, 3, 2, 3, 1, 4, 2, 3, 3, 2, 5, 4, 2, 4, 3, 5, 3, 4, 4, 3, 6, 2, 5, 3, 4, 4, 3, 5, 3, 4, 5, 5, 3, 4, 5, 3, 4, 7, 4, 6, 4, 5, 4, 4, 6, 4, 5, 3, 5, 4, 5, 5, 4, 5, 4, 5, 6, 7, 4, 5, 6, 5, 5, 8, 2, 7, 4, 6, 6, 4, 6, 6, 4, 7, 5, 5, 6, 5, 5, 6, 5, 6, 5, 8, 4, 7, 5, 6, 6, 5, 3, 7, 5, 7]
```
## Mathematica
```Mathematica
a[0] = 0; a[n_] := a[n] = a[Abs[n - 1 - a[n - 1]^2]] + 1; Array[a, 100, 0] (* _Amiram Eldar_, Jul 13 2023 *)
```
## Python
```Python
a = [0]; [a.append(a[abs(n-a[n]**2)]+1) for n in range(100)]
```
