# a\(n\+1\) \= a\(\|n\-a\(n\)\*a\(n\-1\)\|\)\+1; a\(0\) \= 0\.
https://oeis.org/A364663
## JSON
```JSON
[0, 1, 2, 1, 2, 3, 2, 1, 4, 3, 2, 3, 4, 1, 4, 3, 2, 3, 4, 3, 2, 5, 4, 3, 4, 5, 4, 3, 4, 3, 4, 5, 4, 5, 2, 5, 6, 3, 4, 5, 4, 3, 4, 5, 4, 5, 6, 3, 4, 7, 6, 5, 6, 5, 4, 3, 6, 5, 4, 5, 6, 5, 6, 5, 6, 3, 4, 5, 4, 5, 8, 5, 6, 5, 6, 5, 6, 7, 6, 7, 4, 7, 6, 5, 6, 5, 4, 5, 6, 5, 6, 7, 8, 7, 4, 5, 6]
```
## Python
```Python
a=[0];
for n in range(100):
    a.append(a[abs(n-a[n]*a[n-1])]+1)
```
## PARI
```PARI
N=100; a=vector(N); a[2]=1; for(n=1,N-2,a[n+2]=a[1+abs(n-a[n]*a[n+1])]+1);
```
