# Descending dungeons: see Comments lines for definition\.
https://oeis.org/A121263
## JSON
```JSON
[10, 11, 13, 16, 20, 25, 31, 38, 46, 55, 65, 87, 135, 239, 463, 943, 1967, 4143, 8751, 18479, 38959, 103471, 306223, 942127, 2932783, 9153583, 28562479, 89028655, 277145647, 861652015, 2675637295, 10173443119, 41132125231, 168836688943, 695134284847]
```
## Maple
```Maple
M:=100; a:=list(10..M): a[10]:=10: lprint(10,a[10]); for n from 11 to M do b:=n; for i from n-1 by -1 to 11 do t1:=convert(i,base,10); b:=add(t1[j]*b^(j-1),j=1..nops(t1)): od: a[n]:=b; lprint(n,a[n]); od: # _N. J. A. Sloane_
asubb := proc(a,b) local t1; t1:=convert(a,base,10); add(t1[j]*b^(j-1),j=1..nops(t1)): end; # asubb(a,b) evaluates a as if it were written in base b # _N. J. A. Sloane_
```
## Python
```Python
def a(n):
  a_of_n = [((10 + int(i))) for i in range(n)]
  while len(a_of_n) != 1:
    exponent = 0
    a_of_n [-2] = list(str(a_of_n [-2]))
    for i in range(len(a_of_n [-2])):
      a_of_n [-2] [-(i+1)] = int(a_of_n [-2] [-(i+1)])
      a_of_n [-2] [-(i+1)] *= ((a_of_n [-1]) ** exponent)
      exponent += 1
    a_of_n [-2] = sum(a_of_n [-2])
    a_of_n = a_of_n [:((len(a_of_n))-1)]
  return (a_of_n [0])
# _Noah J. Crandall_, Dec 07 2020
```
