# a\(n\) \= Sum\_\{k\=1\.\.n\} n\! \* n^\(n\-k\+1\) / \(n\-k\)\!\.
https://oeis.org/A036360
## JSON
```JSON
[0, 1, 12, 153, 2272, 39225, 776736, 17398969, 435538944, 12058401393, 366021568000, 12090393761721, 431832459644928, 16585599200808937, 681703972229640192, 29858718555221585625, 1388451967046195347456, 68316647610168842824161, 3546179063131198669848576, 193670918442059606406896473]
```
## Maple
```Maple
a := proc(n) local k; add(n!*n^(n-k+1)/(n-k)!, k=0..n); end;
# Alternative, e.g.f.:
T := -LambertW(-x): egf := (T + T^2)/(1 - T)^4: ser := series(egf, x, 22):
seq(n!*coeff(ser, x, n), n = 0..19);  # _Peter Luschny_, Jul 20 2024
```
## Mathematica
```Mathematica
Table[Sum[n!*n^(n-k+1)/(n-k)!, {k, 1, n}], {n, 0, 19}] (* _James C. McMahon_, Feb 07 2024 *)
```
```Mathematica
a[n_] := n E^n Gamma[n + 1, n] - n^(n + 1);
```
```Mathematica
Table[a[n], {n, 0, 19}]  (* _Peter Luschny_, Jul 20 2024 *)
```
## Python
```Python
def a(n):
    total_sum = 0
    for k in range(1, n + 1):
        term = (math.factorial(n) / math.factorial(n - k))*(k**2)*(n**(n - k))
        total_sum += term
    return total_sum
# _Brian P Hawkins_, Jan 06 2024
```
## PARI
```PARI
a(n) = sum(k=1, n, n! * n^(n-k+1) / (n-k)!) \\ _Andrew Howroyd_, Jan 06 2024
```
