# n\-th term of the Fibonacci\-type sequence x\(1\)\=1, x\(2\)\=Fibonacci\(n\), x\(k\+1\)\=x\(k\)\+x\(k\-1\) for k\>1\.
https://oeis.org/A142975
## JSON
```JSON
[1, 1, 3, 7, 17, 43, 109, 281, 727, 1891, 4929, 12871, 33641, 87985, 230203, 602447, 1576849, 4127635, 10805301, 28287049, 74053871, 193871371, 507555073, 1328785487, 3478787857, 9107556193, 23843845299, 62423922391, 163427829137, 427859414971, 1120150172989]
```
## Maple
```Maple
F:= combinat[fibonacci]:
seq(F(n-1)*F(n)+F(n-2), n=1..32);
```
## Mathematica
```Mathematica
fts[{a_,b_,c_}]:=b*c+a; fts/@Partition[Fibonacci[Range[-1,30]],3,1] (* or *) LinearRecurrence[ {3,1,-5,-1,1},{1,1,3,7,17},40] (* _Harvey P. Dale_, Nov 24 2016 *)
```
## Python
```Python
def fib(arb1,arb2,nth):
    if nth == 0:
            return arb1
    if nth == 1:
            return arb2
    x = [0]*nth
    x[0] = arb1
    x[1] = arb2
    for i in range(2,nth,1):
            x[i] = x[i-1]+x[i-2]
    return x[-1]
def fib2d(n):
    return fib(1,fib(1,1,n),n)
[fib2d(i) for i in range(1,10)]
# the function fib2d will return the n-th term of the sequence.
```
