# a\(n\) \= phi\(n\) \- phi\(n\-phi\(n\)\), a\(1\) \= 1\.
https://oeis.org/A346692
## JSON
```JSON
[1, 0, 1, 1, 3, 0, 5, 2, 4, 2, 9, 0, 11, 2, 2, 4, 15, 2, 17, 4, 6, 6, 21, 0, 16, 6, 12, 4, 27, -2, 29, 8, 8, 10, 14, 4, 35, 10, 16, 8, 39, 4, 41, 12, 12, 14, 45, 0, 36, 12, 14, 12, 51, 6, 32, 8, 24, 20, 57, -4, 59, 14, 18, 16, 32, -2, 65, 20, 24, 2, 69, 8, 71, 18, 16, 20, 44, 6, 77, 16]
```
## Maple
```Maple
with(numtheory):
A := seq(phi(n) - phi(n-phi(n)), n=1..100);
```
## Mathematica
```Mathematica
a[n_] := (phi = EulerPhi[n]) - EulerPhi[n - phi]; Array[a, 100] (* _Amiram Eldar_, Jul 29 2021 *)
```
## PARI
```PARI
a(n) = if (n==1, 1, eulerphi(n) - eulerphi(n-eulerphi(n))); \\ _Michel Marcus_, Jul 29 2021
```
## Python
```Python
from sympy import totient as phi
def a(n):
    if n == 1: return 1
    phin = phi(n)
    return phin - phi(n - phin)
print([a(n) for n in range(1, 81)]) # _Michael S. Branicky_, Jul 29 2021
```
