# If n \= Sum\_\{i\=0\.\.m\} c\(i\)\*2^i, c\(i\) \= 0 or 1, then a\(n\) \= Sum\_\{i\=0\.\.m\} \(m\+1\-i\)\*c\(i\)\.
https://oeis.org/A230877
## JSON
```JSON
[0, 1, 1, 3, 1, 4, 3, 6, 1, 5, 4, 8, 3, 7, 6, 10, 1, 6, 5, 10, 4, 9, 8, 13, 3, 8, 7, 12, 6, 11, 10, 15, 1, 7, 6, 12, 5, 11, 10, 16, 4, 10, 9, 15, 8, 14, 13, 19, 3, 9, 8, 14, 7, 13, 12, 18, 6, 12, 11, 17, 10, 16, 15, 21, 1, 8, 7, 14, 6, 13, 12, 19, 5, 12, 11, 18, 10, 17, 16, 23, 4, 11, 10, 17, 9, 16, 15, 22, 8, 15, 14]
```
## Maple
```Maple
f:=proc(n) local t1,m,i;
t1:=convert(n,base,2);
m:=nops(t1)-1;
add((m+1-i)*t1[i+1], i=0..m);
end;
```
## Mathematica
```Mathematica
Array[Total[Position[IntegerDigits[#, 2], 1], 2] &, 100, 0] (* _Paolo Xausa_, Mar 18 2024 *)
```
## PARI
```PARI
a(n) = { my (b=binary(n)); sum(k=1, #b, b[k]*k) } \\ _RÃ©my Sigrist_, Jun 25 2021
```
## Python
```Python
def A230877(n): return sum(i for i, j in enumerate(bin(n)[2:],1) if j=='1') # _Chai Wah Wu_, Jan 09 2023
```
