# a\(n\) \= sum\{k\=1 to n\} \(A114112\(k\)\)\. \(For n\>\=2, a\(n\) \= sum\{k\=1 to n\} \(A014681\(k\)\) \=sum\{k\=1 to n\} \(A103889\(k\)\)\.\)\.
https://oeis.org/A114113
## JSON
```JSON
[1, 3, 7, 10, 16, 21, 29, 36, 46, 55, 67, 78, 92, 105, 121, 136, 154, 171, 191, 210, 232, 253, 277, 300, 326, 351, 379, 406, 436, 465, 497, 528, 562, 595, 631, 666, 704, 741, 781, 820, 862, 903, 947, 990, 1036, 1081, 1129, 1176, 1226, 1275, 1327, 1378, 1432]
```
## Mathematica
```Mathematica
Join[{1}, LinearRecurrence[{2, 0, -2, 1}, {3, 7, 10, 16}, 52]] (* _Jean-Fran√ßois Alcover_, Sep 22 2017 *)
```
```Mathematica
CoefficientList[Series[(1 + x + x^2 -2 x^3 + x^4)/((1 + x) (1 - x)^3), {x, 0, 60}], x] (* _Vincenzo Librandi_, Mar 13 2018 *)
```
## Magma
```Magma
I:=[1,3,7,10,16]; [n le 5 select I[n] else 2*Self(n-1)-2*Self(n-3)+Self(n-4): n in [1..60]]; // _Vincenzo Librandi_, Mar 13 2018
```
## Python
```Python
def A114113(n): return 1 if n == 1 else (m:=n//2)*(n+1) + (n+1-m)*(n-2*m) # _Chai Wah Wu_, May 24 2022
```
