# Recurrence a\(n\+2\) \= Sum\_\{k\=0\.\.n\} binomial\(n,k\)\*a\(k\)\*a\(n\+1\-k\) with a\(0\)\=3, a\(1\)\=\-2\.
https://oeis.org/A289069
## JSON
```JSON
[3, -2, -6, -14, -6, 202, 1506, 4594, -29814, -573062, -4098606, 2741026, 487823034, 6657110122, 28995776706, -685482188846, -17937265077654, -181680546169382, 963087154054194, 72085899963332866, 1289184007236331674, 4679677879996688842, -383123191395931184094]
```
## Mathematica
```Mathematica
a[0] = 3; a[1] = -2; a[n_] := a[n] = Sum[Binomial[n - 2, k] a[k] a[n - k - 1], {k, 0, n - 2}]; Array[a, 23, 0] (* _Michael De Vlieger_, Jul 04 2017 *)
```
## PARI
```PARI
c0=3;c1=-2;nmax = 200;
  a=vector(nmax+1);a[1]=c0;a[2]=c1;
  for(m=0,#a-3,a[m+3]=sum(k=0,m,binomial(m,k)*a[k+1]*a[m+2-k]));
  a
```
## Python
```Python
from sympy import binomial
l=[3, -2]
for n in range(2, 51): l+=[sum(binomial(n - 2, k)*l[k]*l[n - 1 - k] for k in range(n - 1)), ]
print(l) # _Indranil Ghosh_, Jun 30 2017
```
