# Recurrence a\(n\+2\) \= Sum\_\{k\=0\.\.n\} binomial\(n,k\)\*a\(k\)\*a\(n\+1\-k\) with a\(0\)\=1, a\(1\)\=\-2\.
https://oeis.org/A289068
## JSON
```JSON
[1, -2, -2, 2, 14, 10, -170, -670, 2270, 30490, 26950, -1435150, -8513650, 59564650, 1050090550, 486517250, -113618013250, -831340535750, 10136160835750, 208459859695250, -121723298991250, -41568491959973750, -338549875950886250, 6637158567781561250]
```
## PARI
```PARI
c0=1;c1=-2;nmax = 200;
  a=vector(nmax+1);a[1]=c0;a[2]=c1;
  for(m=0,#a-3,a[m+3]=sum(k=0,m,binomial(m,k)*a[k+1]*a[m+2-k]));
  a
```
## Python
```Python
from sympy import binomial
l=[1, -2]
for n in range(2, 51): l+=[sum([binomial(n - 2, k)*l[k]*l[n - 1 - k] for k in range(n - 1)]), ]
print(l) # _Indranil Ghosh_, Jun 30 2017
```
