# a\(1\) \= a\(2\) \= a\(3\) \= 2;  a\(n\) \= a\(n\-a\(n\-1\)\) \+ a\(n\-a\(n\-3\)\-1\) for n \> 3\.
https://oeis.org/A289256
## JSON
```JSON
[2, 2, 2, 4, 4, 4, 4, 6, 6, 8, 6, 8, 8, 8, 8, 10, 10, 12, 10, 14, 10, 14, 12, 16, 14, 16, 14, 16, 16, 16, 16, 18, 18, 20, 18, 22, 18, 24, 18, 24, 20, 26, 22, 26, 22, 28, 24, 30, 24, 30, 24, 30, 26, 32, 28, 32, 30, 32, 30, 32, 32, 32, 32, 34, 34, 36, 34, 38, 34, 40, 34, 42, 34, 42, 36, 44, 38, 44, 38, 46, 40, 48]
```
## Mathematica
```Mathematica
a[n_] := a[n] = If[n <= 3, 2, a[n - a[n - 1]] + a[n - a[n - 3] - 1]]; Array[a, 82] (* _Michael De Vlieger_, Jun 30 2017 *)
```
## PARI
```PARI
q=vector(10^5); q[1]=q[2]=q[3]=2;for(n=4, #q, q[n] = q[n-q[n-1]]+q[n-1-q[n-3]]); q
```
## Python
```Python
l=[0, 2, 2, 2]
for n in range(4, 101): l+=[l[n - l[n - 1]] + l[n - l[n - 3] - 1], ]
print(l[1:]) # _Indranil Ghosh_, Jul 01 2017
```
