# a\(n\) \= Sum\_\{k \= 0\.\.n\} \( binomial\(n\+k\-1,k\) \+ binomial\(n\+k\-1,k\)^2 \)\.
https://oeis.org/A357671
## JSON
```JSON
[2, 4, 20, 166, 1812, 22504, 297362, 4067298, 56897300, 809019580, 11649254520, 169444978124, 2485270719570, 36707044807996, 545386321069862, 8144809732228666, 122177690210103060, 1839933274439787940, 27804610626798500372, 421476329345312885304, 6406685025104178888312]
```
## Maple
```Maple
seq(add( binomial(n+k-1,k) + binomial(n+k-1,k)^2, k = 0..n ), n = 0..20);
```
## PARI
```PARI
a(n) = sum(k = 0, n, binomial(n+k-1,k) + binomial(n+k-1,k)^2); \\ _Michel Marcus_, Oct 24 2022
```
## Python
```Python
from math import comb
def A357671(n): return comb(n<<1,n)+sum(comb(n+k-1,k)**2 for k in range(n+1)) if n else 2 # _Chai Wah Wu_, Oct 28 2022
```
