# Sequence begins 1, 1, 1; for even n \> 3, a\(n\) \= a\(n/2 \- 1\) \+ a\(n/2 \+ 1\); for odd n \> 3, a\(n\) \= \-a\(\(n\-1\)/2\)\.
https://oeis.org/A359368
## JSON
```JSON
[1, 1, 1, 2, -1, 3, -1, 0, -2, 5, 1, -2, -3, 3, 1, -3, 0, 5, 2, -1, -5, 3, -1, -2, 2, 1, 3, -2, -3, 0, -1, 1, 3, 2, 0, 2, -5, 4, -2, -3, 1, 2, 5, -6, -3, 1, 1, 1, 2, -1, -2, 5, -1, -1, -3, 0, 2, -2, 3, -4, 0, 1, 1, 2, -1, 3, -3, 3, -2, 4, 0, -5, -2, 6, 5, -7, -4, 1, 2, -1]
```
## Mathematica
```Mathematica
a[1]=a[2]=a[3]=1; a[n_]:=If[EvenQ[n],a[n/2-1]+a[n/2+1],-a[(n-1)/2]]; Array[a,80] (* _Stefano Spezia_, Dec 29 2022 *)
```
## Python
```Python
def Seq(n): # generates n terms
    seq = [1,1,1]
    k = 0
    while len(seq) < n:
        seq += [seq[k] + seq[k+2]]
        seq += [-1*seq[k+1]]
        k += 1
    return seq
```
