# Expansion of Sum\_\{k\>\=1\} x^k/\(1 \- x^k \- 2\*x^\(2\*k\)\)\.
https://oeis.org/A309729
## JSON
```JSON
[1, 2, 4, 7, 12, 26, 44, 92, 175, 354, 684, 1396, 2732, 5506, 10938, 21937, 43692, 87578, 174764, 349884, 699098, 1398786, 2796204, 5593886, 11184823, 22372354, 44739418, 89483996, 178956972, 357925242, 715827884, 1431677702, 2863312218, 5726666754, 11453246178, 22906581193]
```
## Maple
```Maple
seq(add(2^d-(-1)^d, d=numtheory:-divisors(n))/3, n=1..50); # _Robert Israel_, Aug 14 2019
```
## Mathematica
```Mathematica
nmax = 36; CoefficientList[Series[Sum[x^k/(1 - x^k - 2 x^(2 k)), {k, 1, nmax}], {x, 0, nmax}], x] // Rest
```
```Mathematica
Table[(1/3) Sum[(2^d - (-1)^d), {d, Divisors[n]}], {n, 1, 36}]
```
## PARI
```PARI
a(n)={sumdiv(n, d, 2^d - (-1)^d)/3} \\ _Andrew Howroyd_, Aug 14 2019
```
## Python
```Python
n = 1
while n <= 36:
    s, d = 0, 1
    while d <= n:
        if n%d == 0:
            s = s+2**d-(-1)**d
        d = d+1
    print(n,s//3)
n = n+1 # _A.H.M. Smeets_, Aug 14 2019
```
