# a\(n\) \= a\(n\-1\) \* a\(n\-2\) \+ 1 if n is even, otherwise a\(n\) \= a\(n\-3\) \+ 1, with a\(0\) \= a\(1\) \= 1\.
https://oeis.org/A356891
## JSON
```JSON
[1, 1, 2, 2, 5, 3, 16, 6, 97, 17, 1650, 98, 161701, 1651, 266968352, 161702, 43169316455105, 266968353, 11524841314155180292066, 43169316455106, 497519521785644682185076928856988997, 11524841314155180292067]
```
## Mathematica
```Mathematica
a[n_] := a[n] = If[EvenQ[n], a[n - 1]*a[n - 2], a[n - 3]] + 1; a[0] = a[1] = 1; Array[a, 22, 0] (* _Amiram Eldar_, Sep 10 2022 *)
```
## Python
```Python
def A356891(length):
    output = [1] * length
    for n in range(2, length):
        output[n] += output[n-3] if n % 2 else output[n-1] * output[n-2]
    return output
```
