# a\(n\+1\) \= \(a\(n\) \- 2\*\(n\-1\)\) \* \(2\*n\-1\), where a\(1\)\=1\.
https://oeis.org/A339516
## JSON
```JSON
[1, 1, -3, -35, -287, -2655, -29315, -381251, -5718975, -97222847, -1847234435, -38791923555, -892214242271, -22305356057375, -602244613549827, -17465093792945795, -541417907581320575, -17866790950183580031, -625337683256425302275, -23137494280487736185507]
```
## Maple
```Maple
A339516 := proc(n)
    option remember ;
    if n = 1 then
        1;
    else
        (2*n-3)*(procname(n-1)-2*(n-2)) ;
    end if;
end proc:
seq(A339516(n),n=1..30) ; # _R. J. Mathar_, Aug 24 2022
```
## Mathematica
```Mathematica
a[1]=1;a[n_]:=(a[n-1]-2(n-2))(2n-3); Array[a,20] (* _Stefano Spezia_, Dec 08 2020 *)
```
```Mathematica
nxt[{n_,a_}]:={n+1,(a-2n)(2n+1)}; Join[{1},NestList[nxt,{1,1},20][[;;,2]]] (* _Harvey P. Dale_, Aug 25 2024 *)
```
## Python
```Python
#generate first 50 numbers of the sequence
cnt = 50
i=0
seq = list()
seq.append(1)
i=1
while (i<cnt):
    seq.append((seq[i-1]-2*(i-1))*(2*i-1))
    i=i+1
print(seq)
```
