# a\(n\+1\) \= a\(n\-3\-a\(n\)^2\) \+ 1, starting with a\(1\) \= a\(2\) \= a\(3\) \= a\(4\) \= 0\.
https://oeis.org/A339931
## JSON
```JSON
[0, 0, 0, 0, 1, 1, 1, 1, 1, 2, 1, 2, 2, 2, 2, 2, 2, 3, 2, 3, 2, 3, 3, 2, 3, 3, 3, 3, 3, 3, 4, 3, 4, 3, 4, 3, 3, 4, 3, 4, 3, 4, 4, 3, 4, 4, 4, 4, 4, 4, 5, 4, 5, 4, 5, 4, 4, 5, 4, 5]
```
## Python
```Python
a = [0, 0, 0, 0]
for n in range(3, 1000):
    a.append(a[n-3-a[n]**2]+1)
```
## C
```C
#include<stdio.h>
#include<stdlib.h>
int main(void){
    int N = 1000;
    int *a = (int*)malloc(N*sizeof(int));
    a[0] = 0;
    a[1] = 0;
    a[2] = 0;
    a[3] = 0;
    for(int n = 3; n < N-1; ++n){
        a[n+1] = a[n-3-a[n]*a[n]]+1;
    }
    free(a);
    return 0;
}
```
