# The Bodlaender function: a\(1\) \= \-1; a\(2\*n\) \= a\(n\), a\(2\*n\+1\) \= a\(n\+1\) \+ n\.
https://oeis.org/A354158
## JSON
```JSON
[-1, -1, 0, -1, 2, 0, 2, -1, 6, 2, 5, 0, 8, 2, 6, -1, 14, 6, 11, 2, 15, 5, 11, 0, 20, 8, 15, 2, 20, 6, 14, -1, 30, 14, 23, 6, 29, 11, 21, 2, 35, 15, 26, 5, 33, 11, 23, 0, 44, 20, 33, 8, 41, 15, 29, 2, 48, 20, 35, 6, 44, 14, 30, -1, 62, 30, 47, 14, 57, 23, 41, 6, 65, 29, 48, 11, 59, 21, 41, 2, 75, 35, 56, 15, 68, 26, 48, 5, 77, 33]
```
## Maple
```Maple
g:=proc(n) option remember; if n = 1 then -1 elif (n mod 2) = 0 then g(n/2) else (n-1)/2 + g((n+1)/2); fi; end;
```
## Python
```Python
from functools import lru_cache
@lru_cache(maxsize=None)
def a(n):
    if n == 1: return -1
    return a(n//2+1) + n//2 if n&1 else a(n//2)
print([a(n) for n in range(1, 91)]) # _Michael S. Branicky_, Jul 25 2022
```
