# a\(n\) \= a\(n\-1\) \+ a\(n\-2\) \+ 2\*a\(n\-3\) with a\(0\)\=2, a\(1\)\=1, a\(2\)\=5\.
https://oeis.org/A226308
## JSON
```JSON
[2, 1, 5, 10, 17, 37, 74, 145, 293, 586, 1169, 2341, 4682, 9361, 18725, 37450, 74897, 149797, 299594, 599185, 1198373, 2396746, 4793489, 9586981, 19173962, 38347921, 76695845, 153391690, 306783377, 613566757, 1227133514, 2454267025, 4908534053, 9817068106, 19634136209]
```
## Maple
```Maple
A226308 := n -> 1/7*(2^(n+3) + 6*cos(2*Pi*n/3) - 4*sqrt(3)*sin(2*Pi*n/3)):
seq(A226308(n), n = 0 .. 34); # _MÃ©lika Tebni_, Mar 09 2024
```
## Mathematica
```Mathematica
CoefficientList[Series[-(2 x^2 - x + 2) / ((2 x - 1) (x^2 + x + 1)), {x, 0, 40}], x] (* _Vincenzo Librandi_, Jun 18 2013 *)
```
## Python
```Python
a0, a1, a2 = 2, 1, 5
for n in range(77):
  a = a2 + a1 + 2*a0
  print(a0, end=', ')
  a0, a1, a2 = a1, a2, a # _Alex Ratushnyak_, Jun 08 2013
```
## PARI
```PARI
a(n)=([0,1,0; 0,0,1; 2,1,1]^n*[2;1;5])[1,1] \\ _Charles R Greathouse IV_, Jul 19 2016
```
