# a\(0\) \= 0; a\(1\) \= 1; a\(2\*n\) \= 2\*a\(n\), a\(2\*n\+1\) \= 2\*a\(n\) \+ \(\-1\)^a\(n\+1\)\.
https://oeis.org/A283165
## JSON
```JSON
[0, 1, 2, 3, 4, 3, 6, 7, 8, 7, 6, 7, 12, 11, 14, 15, 16, 15, 14, 15, 12, 11, 14, 15, 24, 23, 22, 23, 28, 27, 30, 31, 32, 31, 30, 31, 28, 27, 30, 31, 24, 23, 22, 23, 28, 27, 30, 31, 48, 47, 46, 47, 44, 43, 46, 47, 56, 55, 54, 55, 60, 59, 62, 63, 64, 63, 62, 63, 60, 59, 62, 63, 56, 55, 54, 55, 60, 59, 62, 63, 48, 47, 46, 47, 44, 43, 46, 47, 56, 55, 54]
```
## Mathematica
```Mathematica
a[0] = 0; a[1] = 1; a[n_] := If[EvenQ[n], 2 a[n/2], 2 a[(n - 1)/2] + (-1)^a[(n + 1)/2]]; Table[a[n], {n, 0, 90}]
```
## PARI
```PARI
a(n) = if (n<2, n, if (n%2==0, 2*a(n/2), 2*a((n-1)/2)+(-1)^(a(n+1)/2)));
tabl(nn)={for (n=0, nn, print1(a(n), ", "); ); };
tabl(90); \\ _Indranil Ghosh_, Mar 03 2017
```
## Python
```Python
def a(n):
....if n<2: return n
....if n%2==0: return 2*a(n/2)
....else: return 2*a((n-1)/2)+(-1)**a((n+1)/2) # _Indranil Ghosh_, Mar 03 2017
```
