# a\(n\) \= A285735\(n\) \- A285734\(n\) \= n \- 2\*A285734\(n\)\.
https://oeis.org/A285736
## JSON
```JSON
[1, 0, 1, 0, 1, 0, 3, 2, 3, 0, 1, 0, 1, 0, 5, 4, 3, 4, 7, 0, 1, 0, 3, 2, 3, 0, 1, 0, 1, 0, 3, 2, 5, 0, 7, 2, 7, 0, 5, 2, 3, 0, 1, 0, 1, 0, 5, 4, 3, 8, 7, 0, 7, 8, 3, 4, 5, 0, 1, 0, 1, 0, 3, 2, 3, 0, 1, 0, 1, 0, 3, 2, 3, 0, 1, 0, 1, 0, 3, 2, 3, 0, 1, 0, 1, 0, 5, 4, 3, 4, 15, 0, 1, 0, 11, 10, 5, 4, 7, 6, 9, 0, 11, 2, 11, 0, 15, 2, 7, 0, 5, 2, 3, 0, 1, 0, 1, 0, 3]
```
## Scheme
```Scheme
(define (A285736 n) (- (A285735 n) (A285734 n)))
(define (A285736 n) (- n (* 2 (A285734 n))))
```
## Python
```Python
from sympy.ntheory.factor_ import core
def issquarefree(n): return core(n) == n
def a285734(n):
    if n==1: return 0
    j=n//2
    while True:
        if issquarefree(j) and issquarefree(n - j): return j
        else: j-=1
def a285736(n): return n - 2*a285734(n)
print([a285736(n) for n in range(1, 101)]) # _Indranil Ghosh_, May 02 2017
```
