# T\(n, k\) \= binomial\(2\*n \- 1 \- k, k \- 1\)\*hypergeom\(\[2, 2, 1\-k\], \[1, 1 \- 2\*k \+ 2\*n\], \-1\), triangle read by rows, T\(n, k\) for n \>\= 1 and 1 <\= k <\= n\.
https://oeis.org/A320905
## JSON
```JSON
[1, 1, 5, 1, 7, 18, 1, 9, 31, 56, 1, 11, 48, 111, 160, 1, 13, 69, 198, 351, 432, 1, 15, 94, 325, 699, 1023, 1120, 1, 17, 123, 500, 1280, 2223, 2815, 2816, 1, 19, 156, 731, 2186, 4458, 6562, 7423, 6912, 1, 21, 193, 1026, 3525, 8330, 14198, 18324, 18943, 16640]
```
## Maple
```Maple
T := (n, k) -> binomial(2*n-1-k,k-1)*hypergeom([2,2,1-k], [1,1-2*k+2*n], -1):
seq(seq(simplify(T(n, k)), k=1..n), n=1..10);
```
## Mathematica
```Mathematica
T[n_, k_] := Sum[Binomial[2*n-k, 2*n-2*k+1+j]*Binomial[j+2, 2],{j, 0, 2*n-k}]; Flatten[Table[T[n, k], {n, 1, 10}, {k, 1, n}]] (* _Detlef Meya_, Dec 31 2023 *)
```
## PARI
```PARI
T(n, k) = {sum(j=0, 2*n-k, binomial(2*n-k, 2*n - 2*k + 1 + j) * binomial(j+2, 2))} \\ _Andrew Howroyd_, Dec 31 2023
```
## Python
```Python
from functools import cache
@cache
def T(n, k):
    if k < 1 or n < 1: return 0
    if k == 1: return 1
    if k == n: return n * (n + 3) * 2**(n - 3)
    return T(n-1, k) + 2*T(n-1, k-1) - T(n-2, k-2)
for n in range(1, 10): print([T(n, k) for k in range(1, n+1)])
# after _Detlef Meya_, _Peter Luschny_, Jan 01 2024
```
