# T\(n, k\) \= binomial\(2\*n \- k, k \- 1\)\*hypergeom\(\[2, 2, 1 \- k\], \[1, 2\*\(1 \- k \+ n\)\], \-1\), triangle read by rows, T\(n,k\) for n \>\= 0 and 0 <\= k <\= n\.
https://oeis.org/A320906
## JSON
```JSON
[0, 0, 1, 0, 1, 6, 0, 1, 8, 24, 0, 1, 10, 39, 80, 0, 1, 12, 58, 150, 240, 0, 1, 14, 81, 256, 501, 672, 0, 1, 16, 108, 406, 955, 1524, 1792, 0, 1, 18, 139, 608, 1686, 3178, 4339, 4608, 0, 1, 20, 174, 870, 2794, 6144, 9740, 11762, 11520]
```
## Maple
```Maple
T := (n, k) -> binomial(2*n-k, k-1)*hypergeom([2, 2, 1-k], [1, 2*(1-k+n)], -1):
seq(seq(simplify(T(n, k)), k=0..n), n=0..9);
```
## Mathematica
```Mathematica
T[n_, k_] := Sum[Binomial[2*n+1-k, 2*n+2-2*k+j]*Binomial[j+2, 2], {j,0, 2*n+1-k}]; Flatten[Table[T[n, k], {n, 0, 15}, {k, 0, n}]] (* _Detlef Meya_, Dec 31 2023 *)
```
## PARI
```PARI
T(n, k) = {sum(j=0, 2*n+1-k, binomial(2*n+1-k, 2*n+2-2*k+j) * binomial(j+2,2))} \\ _Andrew Howroyd_, Dec 31 2023
```
## Python
```Python
from functools import cache
@cache
def T(n, k):
    if k <= 0 or n <= 0: return 0
    if k == 1: return 1
    if k == n: return n * (n + 1) * 2**(n - 2)
    return T(n-1, k) + 2*T(n-1, k-1) - T(n-2, k-2)
for n in range(10): print([T(n, k) for k in range(n + 1)])
# after _Detlef Meya_, _Peter Luschny_, Jan 01 2024
```
