# Antidiagonal triangle T\(n, k\) \= t\(k, n\-k\+1\) where the square array t\(n,k\) is defined by t\(n, k\) \= k\*t\(n\-2, k\) \+ t\(n\-3, k\), t\(0, k\) \= 0, and t\(1, k\) \= t\(2, k\) \= 1, read by rows\.
https://oeis.org/A172371
## JSON
```JSON
[0, 0, 1, 0, 1, 1, 0, 1, 1, 1, 0, 1, 1, 2, 2, 0, 1, 1, 3, 3, 2, 0, 1, 1, 4, 4, 5, 3, 0, 1, 1, 5, 5, 10, 8, 4, 0, 1, 1, 6, 6, 17, 15, 13, 5, 0, 1, 1, 7, 7, 26, 24, 34, 21, 7, 0, 1, 1, 8, 8, 37, 35, 73, 55, 34, 9, 0, 1, 1, 9, 9, 50, 48, 136, 113, 117, 55, 12]
```
## Mathematica
```Mathematica
T[n_, k_]:= T[n, k]= If[n==0, 0, If[n<3, 1, k*T[n-2, k] +T[n-3, k] ]];
```
```Mathematica
Table[T[k, n-k+1], {n, 0, 12}, {k, 0, n}]//Flatten (* modified by _G. C. Greubel_, May 02 2021 *)
```
## Python
```Python
def T(n, k):
    if (n==0): return 0
    elif (n<3): return 1
    else: return k*T(n-2, k) + T(n-3, k)
flatten([[T(k, n-k+1) for k in (0..n)] for n in (0..12)]) # _G. C. Greubel_, May 02 2021
```
