# T\(n,k\) \= \(\(k \+ n\)^2 \- 4\*k \+ 3 \+ \(\-1\)^k \- \(k \+ n \- 2\)\*\(\-1\)^\(k \+ n\)\)/2; n, k \> 0, read by antidiagonals\.
https://oeis.org/A211377
## JSON
```JSON
[1, 3, 4, 2, 5, 6, 8, 9, 12, 13, 7, 10, 11, 14, 15, 17, 18, 21, 22, 25, 26, 16, 19, 20, 23, 24, 27, 28, 30, 31, 34, 35, 38, 39, 42, 43, 29, 32, 33, 36, 37, 40, 41, 44, 45, 47, 48, 51, 52, 55, 56, 59, 60, 63, 64, 46, 49, 50, 53, 54, 57, 58, 61, 62, 65, 66, 68]
```
## Mathematica
```Mathematica
T[n_, k_] := ((k+n)^2 - 4k + 3 + (-1)^k - (k+n-2)(-1)^(k+n))/2;
```
```Mathematica
Table[T[n-k+1, k], {n, 1, 12}, {k, n, 1, -1}] // Flatten (* _Jean-Fran√ßois Alcover_, Nov 29 2018 *)
```
## Python
```Python
t=int((math.sqrt(8*n-7) - 1)/ 2)
i=n-t*(t+1)/2
j=(t*t+3*t+4)/2-n
result=((t+2)**2-4*j+3+(-1)**j-t*(-1)**(t+2))/2
```
