# a\(n\) \= Sum\_\{k\=0\.\.n\} T\(n,k\) where T\(n,k\) \= \(T\(n\-1, k\-1\) \+ T\(n\-1,k\)\)^2\.
https://oeis.org/A337510
## JSON
```JSON
[1, 2, 6, 52, 3854, 21090612, 629815387162156, 561871511512925116799625359336, 446575758106416254441837050759254156476271759098752411181598]
```
## Python
```Python
def r(i):
  t = [[0, 1, 0], [0, 1, 1, 0]]
  for n in range(2, i+1):
    t.append([0])
    for k in range(1, n+2):
      t[n].append((t[n-1][k-1] + t[n-1][k])**2)
    t[n].append(0)
  return(sum(t[i]))
```
