# a\(n\) \= Sum\_\{k \= 0\.\.n\-1\} \(\-1\)^k\*binomial\(n,k\)^2\*binomial\(n\-1,k\)\.
https://oeis.org/A361716
## JSON
```JSON
[0, 1, -3, -8, 45, 126, -840, -2400, 17325, 50050, -378378, -1100736, 8576568, 25069968, -199536480, -585307008, 4732755885, 13919870250, -113936715750, -335813478000, 2775498395670, 8194328596740, -68263497731520, -201822515032320]
```
## Maple
```Maple
seq(add((-1)^k*binomial(n,k)^2*binomial(n-1,k), k = 0..n-1), n = 0..20);
```
## Mathematica
```Mathematica
A361716[n_]:=Sum[(-1)^k*Binomial[n,k]^2Binomial[n-1,k],{k,0,n-1}];Array[A361716,30,0] (* _Paolo Xausa_, Oct 06 2023 *)
```
## PARI
```PARI
a(n) = sum(k = 0, n-1, (-1)^k*binomial(n,k)^2*binomial(n-1,k)); \\ _Michel Marcus_, Mar 26 2023
```
## Python
```Python
from math import comb
def A361716(n): return (sum(comb(n,k)**3*k if k&1 else -comb(n,k)**3*k for k in range(n+1)))//(n if n&1 else -n) if n else 0 # _Chai Wah Wu_, Mar 27 2023
```
