# a\(n\) \= a\(1\)\*a\(n\-1\) \+ a\(2\)\*a\(n\-2\) \+ \.\.\. \+ a\(n\-5\)\*a\(5\) for n \>\= 6, with a\(1\)\=0 and a\(2\)\=a\(3\)\=a\(4\)\=a\(5\)\=1\.
https://oeis.org/A361313
## JSON
```JSON
[0, 1, 1, 1, 1, 0, 1, 1, 2, 3, 4, 8, 11, 20, 31, 52, 88, 143, 247, 408, 700, 1184, 2017, 3462, 5909, 10196, 17518, 30281, 52365, 90704, 157556, 273742, 476893, 831298, 1451603, 2537736, 4441262, 7782934, 13650555, 23969794, 42126241, 74105773, 130476070]
```
## Python
```Python
def A361313(l):
    s = [0, 1, 1, 1, 1][:l]
    for n in range(5, l):
        s.append(sum([s[k] * s[n-k-1] for k in range(n-4)]))
    return s
```
