# a\(0\)\=1, a\(n\) \= \(sum of previous terms\) mod \(a\(n\-1\)\+n\)\.
https://oeis.org/A215451
## JSON
```JSON
[1, 1, 2, 4, 0, 3, 2, 4, 5, 8, 12, 19, 30, 5, 1, 1, 13, 21, 15, 11, 3, 17, 22, 20, 0, 20, 10, 28, 54, 0, 2, 4, 14, 23, 33, 0, 12, 28, 52, 45, 35, 48, 88, 61, 42, 36, 35, 70, 16, 1, 8, 41, 3, 21, 0, 5, 18, 23, 43, 17, 1, 41, 65, 111, 149, 25, 1, 53, 29, 63, 98, 102, 154, 5]
```
## Mathematica
```Mathematica
nxt[{n_,t_,a_}]:=Module[{c=Mod[t,a+n+1]},{n+1,t+c,c}]; NestList[nxt,{0,1,1},80][[All,3]] (* _Harvey P. Dale_, Dec 30 2017 *)
```
## Python
```Python
sum = a = 1
for n in range(1,333):
    print a,
    a = sum % (a+n)
    sum += a
```
