# a\(1\)\=1, a\(n\) \= \(sum of previous terms\) mod \(a\(n\-1\)\+n\)\.
https://oeis.org/A215452
## JSON
```JSON
[1, 1, 2, 4, 8, 2, 0, 2, 9, 10, 18, 27, 4, 16, 11, 7, 2, 4, 13, 9, 0, 18, 4, 4, 2, 10, 3, 5, 26, 54, 21, 32, 4, 29, 42, 14, 10, 44, 57, 44, 63, 6, 5, 10, 52, 23, 32, 44, 64, 74, 71, 33, 18, 60, 93, 29, 46, 48, 60, 84, 38, 26, 39, 46, 83, 81, 25, 59, 93, 22, 47, 24, 34, 53]
```
## Mathematica
```Mathematica
nxt[{t_,n_,a_}]:={t+a,n+1,Mod[t+a,a+n+1]}; NestList[nxt,{0,1,1},80][[All,3]] (* _Harvey P. Dale_, Sep 01 2016 *)
```
## Python
```Python
sum = a = 1
for n in range(2,333):
    print a,
    a = sum % (a+n)
    sum += a
```
