# T\(n,k\) \= \(\(n \+ k \- 1\)\*\(n \+ k \- 2\) \- \(\-1 \+ \(\-1\)^floor\(\(n \+ k\)/2\)\)\*n \+ \(1 \+\(\-1\)^floor\(\(n \+ k\)/2\)\)\*k\)/2; n , k \> 0, read by antidiagonals\.
https://oeis.org/A218890
## JSON
```JSON
[1, 2, 3, 6, 5, 4, 10, 9, 8, 7, 11, 12, 13, 14, 15, 16, 17, 18, 19, 20, 21, 28, 27, 26, 25, 24, 23, 22, 36, 35, 34, 33, 32, 31, 30, 29, 37, 38, 39, 40, 41, 42, 43, 44, 45, 46, 47, 48, 49, 50, 51, 52, 53, 54, 55, 66, 65, 64, 63, 62, 61, 60, 59, 58, 57, 56, 78]
```
## Maple
```Maple
T:=(n,k)->((n+k-1)*(n+k-2)-(-1+(-1)^floor((n+k)/2))*n+(1+(-1)^floor((n+k)/2))*k)/2: seq(seq(T(k,n-k),k=1..n-1),n=1..13); # _Muniru A Asiru_, Dec 13 2018
```
## Mathematica
```Mathematica
T[n_, k_] := ((n+k-1)(n+k-2) - (-1 + (-1)^Floor[(n+k)/2])n + (1 + (-1)^Floor[(n+k)/2]) k)/2;
```
```Mathematica
Table[T[n-k+1, k], {n, 1, 12}, {k, n, 1, -1}] // Flatten (* _Jean-Fran√ßois Alcover_, Dec 06 2018 *)
```
## Python
```Python
t=int((math.sqrt(8*n-7) - 1)/ 2)
i=n-t*(t+1)/2
j=(t*t+3*t+4)/2-n
z=i+j
result=((z-1)*(z-2)-(-1+(-1)**int(z/2))*i+(1+(-1)**int(z/2))*j)/2
```
## Maxima
```Maxima
T(n,k) = ((n + k - 1)*(n + k - 2) - (-1 + (-1)^floor((n + k)/2))*n + (1 +(-1)^floor((n + k)/2))*k)/2$
create_list(T(k, n - k), n, 1, 12, k, 1, n - 1); /* _Franck Maminirina Ramaharo_, Dec 13 2018 */
```
