# a\(0\)\=0, a\(1\)\=a\(2\)\=1; thereafter, a\(n\+1\) \= n^2 \- a\(n\-1\)\.
https://oeis.org/A187093
## JSON
```JSON
[0, 1, 1, 3, 8, 13, 17, 23, 32, 41, 49, 59, 72, 85, 97, 111, 128, 145, 161, 179, 200, 221, 241, 263, 288, 313, 337, 363, 392, 421, 449, 479, 512, 545, 577, 611, 648, 685, 721, 759, 800, 841, 881, 923, 968, 1013, 1057, 1103, 1152, 1201, 1249, 1299, 1352, 1405, 1457]
```
## Maple
```Maple
A000034 := proc(n) op(1+(n mod 2),[1,2]) ; end proc:
A187093 := proc(n) (n^2-1+(-1)^floor(n/2)*A000034(n))/2 ;end proc: # _R. J. Mathar_
```
## Mathematica
```Mathematica
LinearRecurrence[{3, -4, 4, -3, 1}, {0, 1, 1, 3, 8}, 60] (* _Jean-Fran√ßois Alcover_, Mar 30 2020 *)
```
```Mathematica
Join[{0},RecurrenceTable[{a[1]==a[2]==1,a[n+1]==n^2-a[n-1]},a,{n,60}]] (* _Harvey P. Dale_, Jan 05 2023 *)
```
## Python
```Python
print(0, end=',')       # a(-1)=0
prpr = prev = 1         # a(0)=a(1)=1
for n in range(2, 77):
    print(prpr, end=',')
    curr = n*n - prpr   # a(n) = n^2 - a(n-2)
    prpr = prev
    prev = curr
# from _Alex Ratushnyak_, Aug 05 2012
```
## PARI
```PARI
a(n) = (n^2-1+(-1)^(n\2)*(1 + (n % 2)))/2; \\ _Michel Marcus_, Sep 11 2016
```
