# a\(0\) \= a\(1\) \= 1; a\(2\*n\) \= a\(n\) \- a\(n\-1\), a\(2\*n\+1\) \= Sum\_\{k\=0\.\.n\} a\(n\-k\)\.
https://oeis.org/A288310
## JSON
```JSON
[1, 1, 0, 2, -1, 2, 2, 4, -3, 3, 3, 5, 0, 7, 2, 11, -7, 8, 6, 11, 0, 14, 2, 19, -5, 19, 7, 26, -5, 28, 9, 39, -18, 32, 15, 40, -2, 46, 5, 57, -11, 57, 14, 71, -12, 73, 17, 92, -24, 87, 24, 106, -12, 113, 19, 139, -31, 134, 33, 162, -19, 171, 30, 210, -57, 192, 50, 224, -17, 239, 25]
```
## Mathematica
```Mathematica
a[0] = 1; a[1] = 1; a[n_] := a[n] = If[EvenQ[n], a[n/2] - a[(n - 2)/2], Sum[a[(n - 1)/2 - k], {k, 0, (n - 1)/2}]]; Table[a[n], {n, 0, 70}]
```
## Python
```Python
def a(n): return 1 if n<2 else a(n/2) - a(n/2 - 1) if n%2==0 else sum([a((n - 1)/2 - k) for k in range((n + 1)/2)]) # _Indranil Ghosh_, Jun 08 2017
```
