# a\(0\) \= 0; a\(n\) \= a\(a\(n\-1\)\)\-1 mod \(n\+1\) for all n \>\= 1\.
https://oeis.org/A363447
## JSON
```JSON
[0, 1, 0, 3, 2, 5, 4, 1, 0, 9, 8, 11, 10, 7, 0, 15, 14, 17, 16, 13, 6, 3, 2, 23, 22, 1, 0, 27, 26, 29, 28, 25, 0, 33, 32, 35, 34, 31, 24, 21, 2, 41, 40, 1, 0, 45, 44, 47, 46, 43, 0, 51, 50, 53, 52, 49, 42, 39, 20, 5, 4, 1, 0, 63, 62, 65, 64, 61, 0, 69, 68, 71]
```
## Mathematica
```Mathematica
a[0]:=0; a[n_]:=a[n]=Mod[a[a[n-1]]-1, n+1]; Array[a,72,0]
```
## Python
```Python
a = [0]
for i in range(1, 100):
    a.append((a[a[i - 1]] - 1) % (i + 1))
```
